Expanding on PB Bitblast proof tree

LeanCuttingPlanes/Blasting/Blast.lean
@@ -23,20 +23,9 @@ def bbVar (x : BitVec w) : x = bbT (λi↦x[i]) := by
       -- ⊢ x = cons x[s] (bbT fun i => x[↑i])
       sorry
 
-def bbVar0 (x : BitVec 0) : x = bbT ![] := by
-  have r : (λ i => x[i]) = ![] := List.ofFn_inj.mp rfl
-  rw [←r]
-  exact eq_of_getMsbD_eq (congrFun rfl)
-
-def bbVar1 (x : BitVec 1) : x = bbT ![x[0]] := by
-  have r : (λ i => x[i]) = ![x[0]] := List.ofFn_inj.mp rfl
-  rw [←r]
-  exact bbVar x
-
-def bbVar2 (x : BitVec 2) : x = bbT ![x[0],x[1]] := by
-  have r : (λ i => x[i]) = ![x[0],x[1]] := List.ofFn_inj.mp rfl
-  rw [←r]
-  exact bbVar x
+def bbVar0 (x : BitVec 0) : x = bbT ![] := by exact bbVar x
+def bbVar1 (x : BitVec 1) : x = bbT ![x[0]] := by exact bbVar x
+def bbVar2 (x : BitVec 2) : x = bbT ![x[0],x[1]] := by exact bbVar x
 
 #check congrArg
 
@@ -56,4 +45,61 @@ theorem bitblast_and_eq (x y : BitVec 2)
   simp only [Bool.false_eq_true, eq_iff_iff, iff_false, not_and, Bool.not_eq_true, iff_true]
 
   -- ⊢ (x[0] = true → y[0] = false) ∧ x[1] = true ∧ y[1] = true
+  sorry
+
+--##############################################################################################
+--####################              PSEUDO-BOOLEANS              ###############################
+--##############################################################################################
+
+def Fin.toBool [NeZero n] : Fin n → Bool := λ f => f == 1
+def Bool.toFin : Bool → Fin 2 := λ b => b.toNat
+
+def pbbT {w : ℕ} (v : Fin w → Fin 2) : BitVec w := match w with
+| 0     => 0#0
+| (s+1) => cons (if v s = 1 then true else false) (bbT (λi↦ if v i = 1 then true else false))
+
+def pbbVar (x : BitVec w) : x = pbbT (λi↦ x[i].toFin) := by
+  induction w with
+  | zero => exact eq_of_getMsbD_eq (congrFun rfl)
+  | succ s hi =>
+      unfold pbbT
+      simp only [Fin.natCast_eq_last, Fin.getElem_fin, Fin.val_last, Fin.coe_eq_castSucc, Fin.coe_castSucc]
+      -- s : ℕ
+      -- hi : ∀ (x : BitVec s), x = bbT fun i => x[i]
+      -- x : BitVec (s + 1)
+      -- ⊢ x = cons x[s] (bbT fun i => x[↑i])
+      sorry
+
+def pbbVar2 (x : BitVec 2) : x = pbbT ![x[0].toFin,x[1].toFin] := by
+  exact pbbVar x
+
+-- Now let's try blasting to PseudoBoolean inequalities
+theorem pb_bitblast_and_eq (x y : BitVec 2)
+  : (x &&& y = 10#2) := by
+  have i1 := pbbVar2 x
+  set x₀ := x[0].toFin
+  set x₁ := x[1].toFin
+  have i2 := pbbVar2 y
+  set y₀ := y[0].toFin
+  set y₁ := y[1].toFin
+  have i3 : x &&& y = pbbT ![x₀,x₁] &&& pbbT ![y₀,y₁] := Std.Tactic.BVDecide.Reflect.BitVec.and_congr 2 (pbbT ![x₀, x₁]) (pbbT ![y₀, y₁]) x y i1 i2
+
+  set r := x &&& y
+  set r₀ := r[0].toFin
+  set r₁ := r[1].toFin
+
+  have i4' : pbbT ![x₀,x₁] &&& pbbT ![y₀,y₁] = pbbT ![r₀,r₁] ∧ (x₀ - r₀ ≥ 0 ∧ x₁ - r₁ ≥ 0) := sorry
+  have i4 : pbbT ![x₀,x₁] &&& pbbT ![y₀,y₁] = pbbT ![r₀,r₁] := i4'.left
+
+  have i5 : x &&& y = pbbT ![r₀,r₁] := Eq.trans i3 i4
+
+  have i6 : 10#2 = pbbT ![0,1] := rfl -- pbbConst
+
+  have i7 : (x &&& y = 10#2) = (pbbT ![r₀,r₁] = pbbT ![0,1]) := congrFun (congrArg Eq i5) 10#2
+
+  have i8 :  (pbbT ![r₀,r₁] = pbbT ![0,1]) = ((r₁ + 2*r₀) - (1 + 2 * 0) = 0) := by sorry -- pbbEq
+
+  have i9 : (x &&& y = 10#2) = ((r₁ + 2*r₀) - (1 + 2 * 0) = 0) := Eq.trans i7 i8
+
+  rw [i9]
   sorry
